added support for values

TestTask/Basic.lean
@@ -1,25 +1,40 @@
-import Aesop
-import Mathlib.Order.WellFounded
+import Mathlib.Data.Finmap
 
 inductive IntExpr: Type where
 | const: Int → IntExpr
---| val: String → IntExpr
 | add: IntExpr → IntExpr → IntExpr
 | sub: IntExpr → IntExpr → IntExpr
 | mul: IntExpr → IntExpr → IntExpr
+| val: String → IntExpr
 deriving Repr, Inhabited
 
-def basicExpr := IntExpr.add (IntExpr.const 3) (IntExpr.const 5)
+def basicExpr := IntExpr.add (IntExpr.const 3) (IntExpr.val "sp")
 
 #eval basicExpr
 
-def eval: IntExpr → Int
-| .const α => α
-| .add e₁ e₂ => eval e₁ + eval e₂
-| .sub e₁ e₂ => eval e₁ - eval e₂
-| .mul e₁ e₂ => eval e₁ * eval e₂
+abbrev VarMap := Finmap (α := String) (fun _ => Int)
 
-#eval eval basicExpr
+variable {vars: VarMap}
+
+@[reducible]
+def eval: IntExpr → Option Int
+| .const α => do pure α
+| .add e₁ e₂ => do
+  let l ← eval e₁
+  let r ← eval e₂
+  pure (l + r)
+| .sub e₁ e₂ => do
+  let l ← eval e₁
+  let r ← eval e₂
+  pure (l - r)
+| .mul e₁ e₂ => do
+  let l ← eval e₁
+  let r ← eval e₂
+  pure (l * r)
+| .val s => vars.lookup s
+
+#eval eval (vars := List.toFinmap []) basicExpr
+#eval eval (vars := List.toFinmap [⟨"sp", 3⟩]) basicExpr
 
 
 def IntExprMeasure: IntExpr → Nat
@@ -27,6 +42,7 @@ def IntExprMeasure: IntExpr → Nat
 | .add e₁ e₂ => IntExprMeasure e₁ + IntExprMeasure e₂ + 1
 | .sub e₁ e₂ => IntExprMeasure e₁ + IntExprMeasure e₂ + 1
 | .mul e₁ e₂ => IntExprMeasure e₁ + IntExprMeasure e₂ + 1
+| .val _ => 2
 
 theorem pos_measure (exp: IntExpr): 0 < IntExprMeasure exp := by
   induction exp <;> simp [IntExprMeasure]
@@ -36,90 +52,191 @@ mutual
   def stepBinOp
   (constr: IntExpr → IntExpr → IntExpr)
   (fn: Int → Int → Int) (x y: IntExpr)
-  (h_constr: ∀ x y, IntExprMeasure (constr x y) = IntExprMeasure x + IntExprMeasure y + 1): IntExpr :=
+  (h_constr: ∀ x y, IntExprMeasure (constr x y) = IntExprMeasure x + IntExprMeasure y + 1): Option IntExpr :=
   match x, y with
-  | .const val₁, .const val₂ => .const (fn val₁ val₂)
-  | .const val, e₂ => constr (.const val) (step e₂)
-  | e₁, e₂ => constr (step e₁) e₂
+  | .const val₁, .const val₂ => some (.const (fn val₁ val₂))
+  | .const val, e₂ => do
+    let r ← step e₂
+    pure (constr (.const val) r)
+  | e₁, e₂ => do
+    let l ← step e₁
+    pure (constr l e₂)
   termination_by (IntExprMeasure (constr x y) - 1)
   decreasing_by (
     simp [h_constr, IntExprMeasure]
     simp [h_constr]
     apply pos_measure)
 
-  def step (expr: IntExpr): IntExpr := match expr with
-  | .const α => .const α
+  def step (expr: IntExpr): Option IntExpr := match expr with
+  | .const α => some (.const α)
   | .add e₁ e₂ => stepBinOp (.add) (fun x y => x + y) e₁ e₂ (by simp [IntExprMeasure])
   | .sub e₁ e₂ => stepBinOp (.sub) (fun x y => x - y) e₁ e₂ (by simp [IntExprMeasure])
   | .mul e₁ e₂ => stepBinOp (.mul) (fun x y => x * y) e₁ e₂ (by simp [IntExprMeasure])
+  | .val s =>
+    match vars.lookup s with
+    | some val => some (.const val)
+    | none => none
   termination_by (IntExprMeasure expr)
   decreasing_by (all_goals simp [IntExprMeasure])
 end
 
-#eval step basicExpr
-#eval step (step basicExpr)
+#eval step basicExpr (vars := List.toFinmap [])
+#eval step basicExpr (vars := List.toFinmap [⟨"sp", 3⟩])
 
-def step_iter (exp: IntExpr): Nat → IntExpr
+def step_iter (exp: IntExpr): Nat → Option IntExpr
 | 0 => exp
-| .succ n => step_iter (step exp) n
+| .succ n => do
+  let inner ← step exp (vars := vars)
+  let outer ← step_iter inner n
+  pure outer
 
-theorem step_iter_add (exp: IntExpr) (k n: Nat): step_iter exp (k + n) = step_iter (step_iter exp n) k := by
+theorem step_iter_add (exp: IntExpr) (k n: Nat):
+  step_iter exp (k + n) (vars := vars) =
+  (do
+    let inner ← step_iter exp (vars := vars) n
+    let outer ← step_iter inner (vars := vars) k
+    pure outer) := by
   induction n generalizing exp with
   | zero => simp [step_iter]
   | succ k ih =>
-    simp [step_iter]
-    rw [ih (step exp)]
+    simp [step_iter, Option.bind]
+    aesop
 
 theorem decreasing_measure:
-  (∀ α, exp ≠ IntExpr.const α) → (IntExprMeasure (step exp) < IntExprMeasure exp) := by
+  (∀ α, exp ≠ IntExpr.const α) → (
+    (do
+      let res ← step exp (vars := vars)
+      pure (IntExprMeasure res)) < (some (IntExprMeasure exp))) := by
   intro hexp
   induction exp
-  { simp at hexp }
-  all_goals {
-    simp [step, stepBinOp.eq_def, IntExprMeasure]
+  all_goals try {
+    simp [step, stepBinOp.eq_def, IntExprMeasure] at *
     split
-    all_goals try simp [IntExprMeasure]
-    solve_by_elim
-    solve_by_elim }
+    { simp [Option.bind, IntExprMeasure] }
+    { rename_i xih x y val xh yh
+      have xih_res := xih yh
+      simp [Option.bind, IntExprMeasure] at *
+      split at xih_res
+      { simp [*] }
+      simp [*, IntExprMeasure] at *
+      exact xih_res }
+    { rename_i xih yih x y xh yh
+      have xih_res := xih xh
+      simp [Option.bind] at *
+      split at xih_res
+      { simp [*] }
+      simp [*, IntExprMeasure] at *
+      exact xih_res }
+  }
+  { simp at hexp }
+  simp [step, IntExprMeasure] at *
+  simp [Option.bind]
+  split
+  { simp }
+  rename_i heq
+  split at heq
+  simp at heq
+  simp [←heq, IntExprMeasure]
+  simp at heq
 
 theorem step_preserves_eval:
-  eval (step exp) = eval exp := by
-  induction exp <;> simp [step, eval]
-  all_goals {
-    rw [stepBinOp.eq_def]
-    split <;> simp [eval, *] }
+  (do
+    let res ← step exp (vars := vars)
+    let eval_res ← eval res (vars := vars)
+    pure eval_res) = eval exp (vars := vars) := by
+  induction exp
+  { simp [step, eval, Option.bind] }
+  all_goals try {
+    rename_i x y xih yih
+    simp only [eval]
+    simp [step, stepBinOp.eq_def]
+    split
+    { simp [Option.bind, eval] }
+    { simp [Option.bind]
+      simp [Option.bind] at yih
+      rw [←yih]
+      aesop }
+    simp [Option.bind] at *
+    rw [←yih, ←xih]
+    aesop
+    all_goals simp [eval, Option.bind]
+    { simp [heq, ←yih] }
+    { simp [heq, ←yih] }
+    { simp [heq_2, ←yih] }
+    { simp [heq_2, ←yih] }
+    { simp [heq_2, ←yih] }
+    { simp [heq, heq_2] }
+    { simp [heq_3, heq_2] }
+    { simp [heq_3, heq_2] } }
+  simp [eval, Option.bind, step]
+  split <;> aesop
+  simp [eval] at heq_1
+  simp [heq_1]
 
+theorem step_none_eq_eval_none (exp: IntExpr):
+  step exp (vars := vars) = none → eval exp (vars := vars) = none := by
+    induction exp <;> intro hnone
+    all_goals {
+      simp [step, stepBinOp.eq_def, Option.bind, eval] at *
+      try aesop
+    }
+
+omit vars in
 theorem small_step_eval_bound (exp: IntExpr):
-∀ k, IntExprMeasure exp ≤ k + 1 → step_iter exp k = .const (eval exp) := by
-  intro k hk
+∀ svars: VarMap,
+∀ k, IntExprMeasure exp ≤ k + 1 → step_iter exp k (vars := svars) = (do let res ← eval exp (vars := svars); pure (.const res)) := by
+  intro vars k hk
   induction k generalizing exp
   { simp at hk
     cases exp
     { simp [step_iter, eval] }
-    all_goals {
+    all_goals try {
       rename_i a₁
       simp [IntExprMeasure] at hk
       have lemm := pos_measure a₁
-      omega } }
-  rename_i ih
-  rw [step_iter, ih (step exp)]
-  { simp
-    apply step_preserves_eval  }
-  by_cases hexp: ∀ α, exp ≠ IntExpr.const α
-  { have := decreasing_measure hexp
-    omega }
-  simp at hexp
-  let ⟨a, ha⟩ := hexp
-  simp [ha, step, IntExprMeasure]
+      omega }
+    simp [IntExprMeasure] at hk }
+  rename_i n ih
+  rw [step_iter]
+  by_cases const: ∃ α, exp = .const α
+  { rcases const with ⟨α, hconst⟩
+    have ih_const := ih exp (by simp [hconst, IntExprMeasure])
+    simp [Option.bind, hconst, step] at *
+    simp [ih_const] }
+  by_cases sh: ∃ exp₁, step exp (vars := vars) = some exp₁
+  { rcases sh with ⟨exp₁, sh⟩
+    have dec_measure := decreasing_measure (exp := exp) (vars := vars) (by aesop)
+    simp [Option.bind, sh] at dec_measure
+    have ih_exp := ih (exp₁) (by omega)
+    simp [Option.bind, sh, ih_exp]
+    have preservation := step_preserves_eval (exp := exp) (vars := vars)
+    simp [sh] at preservation
+    simp [←preservation]
+    by_cases heval: ∃ ev, eval exp₁ (vars := vars) = some ev
+    { rcases heval with ⟨ev, heval⟩
+      simp [heval] }
+    simp [←Option.eq_none_iff_forall_ne_some] at heval
+    simp [heval] }
+  simp at *
+  rw [←Option.eq_none_iff_forall_ne_some] at sh
+  simp [Option.bind, sh]
+  simp [step_none_eq_eval_none exp sh]
 
-
+omit vars in
 theorem small_step_eval_seq (exp: IntExpr):
-∃ seq: List IntExpr,
+∀ svars: VarMap,
+∃ seq: List (Option IntExpr),
 1 ≤ seq.length ∧
 seq[0]! = exp ∧
-seq.getLast! = .const (eval exp) ∧
-∀ i < seq.length - 1, seq[i + 1]! = step seq[i]! := by
-  exists (List.range (IntExprMeasure exp)).map (step_iter exp)
+seq.getLast! = (do let evalRes ← eval exp (vars := svars); pure (.const evalRes)) ∧
+∀ i < seq.length - 1,
+  seq[i + 1]! =
+    (do
+      let preSeq ← seq[i]!
+      let preRes ← step preSeq (vars := svars)
+      pure preRes) := by
+  intro vars
+  exists (List.range (IntExprMeasure exp)).map (step_iter exp (vars := vars))
   have := pos_measure exp
   repeat' constructor
   { simp; omega }
@@ -140,15 +257,13 @@ seq.getLast! = .const (eval exp) ∧
   intro i hi
   simp at hi
   simp
-  rw [List.getElem?_eq_getElem]
-  rw [List.getElem?_eq_getElem]
+  repeat rw [List.getElem?_eq_getElem]
   simp
-  rw [List.getElem_range]
-  { rw [List.getElem_range]
-    { rw [step_iter]
-      have := step_iter_add exp 1 i
-      simp [step_iter] at this
-      rw [←this, Nat.add_comm]
-      simp [step_iter] }
-    simp; omega }
+  repeat rw [List.getElem_range]
+  { rw [step_iter]
+    have := step_iter_add exp 1 i (vars := vars)
+    simp [step_iter] at this
+    rw [←this, Nat.add_comm]
+    simp [step_iter] }
+  { simp; omega }
   simp; omega
